Début des preuves de bases sur la prouvabilité.

src/HOL/Theorie.v
@@ -1,10 +1,10 @@
 From CRM Require Import Base Typing fintype.
 Import CombineNotations SubstNotations.
 
-From Stdlib Require Import PeanoNat List Datatypes.
+Require Import PeanoNat List Datatypes Program.Equality.
 Import ListNotations.
 
-Reserved Notation "Γ | Ξ ⊢ φ" (at level 85).
+(*Reserved Notation "Γ | Ξ ⊢⟨ n ⟩ φ" (at level 88).*)
 
 Definition shift11 {n : nat} (g : fin (S n)) : fin (S (S n)).
 Proof.
@@ -23,49 +23,201 @@ Proof.
   apply H.
 Qed.
 
-Definition ex_tm {n : nat} (φ : tm (S n)) : tm n.
+Definition ex_tm {n : nat} (s : st) (φ : tm (S n)) : tm n.
 Proof.
-  apply forall_tm. apply imp_tm.
-  apply forall_tm. apply imp_tm.
+  apply forall_tm. apply ℙₛ. apply imp_tm.
+  apply forall_tm. apply s. apply imp_tm.
   exact (ren_tm shift11 φ). apply var_tm. apply Some. apply None.
   apply var_tm. apply None.
 Defined.
 
-Notation "∃ₛ" := (ex_tm).
+Notation "∃ₛ" := (ex_tm) (at level 80).
 
 Lemma typ_ex_tm : forall (n : nat) (Γ : HOL_ctx n) (s : st) (φ : tm (S n)),
-    s .: Γ ⊢⟨ S n ⟩ φ ~: ℙₛ -> Γ ⊢⟨ n ⟩ ex_tm φ ~: ℙₛ.
+    s .: Γ ⊢⟨ S n ⟩ φ ~: ℙₛ -> Γ ⊢⟨ n ⟩ ∃ₛ s φ ~: ℙₛ.
 Proof.
-  intros. apply (typ_forall ℙₛ).
-  constructor. apply (typ_forall s). constructor.
+  intros. apply typ_forall.
+  constructor. apply typ_forall. constructor.
   apply typ_shift. apply H.
   constructor. constructor.
 Qed.
 
-Definition eq_tm {n : nat} (t : tm n) (u : tm n) : tm n.
+Definition eq_tm {n : nat} (s : st) (t : tm n) (u : tm n) : tm n.
 Proof.
-  apply forall_tm. apply imp_tm.
+  apply forall_tm. apply (s →ₛ ℙₛ). apply imp_tm.
   apply app_tm. apply var_tm; apply None.
   exact (ren_tm shift t).
   apply app_tm. apply var_tm; apply None.
   exact (ren_tm shift u).
 Defined.
 
-Notation "t =ₛ u" := (eq_tm t u) (at level 86).
+Notation "t =⟨ s ⟩ u" := (eq_tm s t u) (at level 77).
 
 Lemma typ_eq_tm : forall (n : nat) (Γ : HOL_ctx n) (s : st)
                          (t : tm n) (u : tm n),
-    Γ ⊢⟨ n ⟩ t ~: s -> Γ ⊢⟨ n ⟩ u ~: s -> Γ ⊢⟨ n ⟩ t =ₛ u ~: ℙₛ.
+    Γ ⊢⟨ n ⟩ t ~: s -> Γ ⊢⟨ n ⟩ u ~: s -> Γ ⊢⟨ n ⟩ t =⟨ s ⟩ u ~: ℙₛ.
 Proof.
-  intros. apply (typ_forall (s →ₛ ℙₛ)).
+  intros. apply typ_forall.
   constructor. apply (typ_app s).
   constructor. apply typ_weaken. apply H.
   apply (typ_app s). constructor. apply typ_weaken. apply H0.
 Qed.
 
-Definition proof_ctx (n : nat) (Γ : fin n -> st) := list (tm n).
+Definition or_tm {n : nat} (t u : tm n) : tm n.
+Proof.
+  apply forall_tm. apply ℙₛ. apply imp_tm.
+  apply imp_tm.
+  exact (ren_tm shift t). apply var_tm. apply None.
+  apply imp_tm. apply imp_tm.
+  exact (ren_tm shift u). apply var_tm. apply None.
+  apply var_tm. apply None.
+Defined.
 
-Inductive wt_ctx {n : nat} {Γ : fin n -> st} : proof_ctx n -> Prop :=
+Notation "φ ∨ₛ ψ" := (or_tm φ ψ) (at level 80).
+
+Lemma typ_eq_or : forall (n : nat) (Γ : HOL_ctx n) (t u : tm n),
+    Γ ⊢⟨ n ⟩ t ~: ℙₛ -> Γ ⊢⟨ n ⟩ u ~: ℙₛ -> Γ ⊢⟨ n ⟩ t ∨ₛ u ~: ℙₛ.
+Proof.
+  intros. apply typ_forall. constructor.
+  constructor. apply typ_weaken. apply H.
+  constructor. constructor. constructor. apply typ_weaken.
+  apply H0. constructor. constructor.
+Qed.
+
+Definition and_tm {n : nat} (t u : tm n) : tm n.
+Proof.
+  apply forall_tm. apply ℙₛ. apply imp_tm. apply imp_tm.
+  apply (ren_tm shift t).
+  apply imp_tm. apply (ren_tm shift u). apply var_tm. apply None.
+  apply var_tm. apply None.
+Defined.
+
+Notation "φ ∧ₛ ψ" := (and_tm φ ψ) (at level 79).
+
+Lemma typ_and : forall (n : nat) (Γ : HOL_ctx n) (φ ψ : tm n),
+    Γ ⊢⟨ n ⟩ φ ~: ℙₛ -> Γ ⊢⟨ n ⟩ ψ ~: ℙₛ -> Γ ⊢⟨ n ⟩ φ ∧ₛ ψ ~: ℙₛ.
+Proof.
+  intros. constructor.
+  constructor. constructor. apply typ_weaken. apply H.
+  constructor. apply typ_weaken. apply H0.
+  constructor. constructor.
+Qed.
+
+Definition true_tm {n : nat} : tm n.
+Proof.
+  apply forall_tm. apply ℙₛ. apply imp_tm. apply var_tm. apply None.
+  apply var_tm. apply None.
+Defined.
+
+Notation "⊤ₛ" := (true_tm).
+
+Lemma typ_true : forall (n : nat) (Γ : HOL_ctx n),
+    Γ ⊢⟨ n ⟩ ⊤ₛ ~: ℙₛ.
+Proof.
+  intros. apply (typ_forall ℙₛ). repeat constructor.
+Qed.
+
+Definition false_tm {n : nat} : tm n.
+Proof.
+  apply forall_tm. apply ℙₛ. apply var_tm. apply None.
+Defined.
+
+Notation "⊥ₛ" := (false_tm).
+
+Lemma typ_false : forall (n : nat) (Γ : HOL_ctx n),
+    Γ ⊢⟨ n ⟩ ⊥ₛ ~: ℙₛ.
+Proof.
+  intros. apply (typ_forall ℙₛ). constructor.
+Qed.
+
+Definition not_tm {n : nat} (t : tm n) : tm n.
+Proof.
+  apply imp_tm. apply t. apply ⊥ₛ.
+Defined.
+
+Notation "¬ₛ φ" := (not_tm φ) (at level 79).
+
+Lemma typ_not : forall (n : nat) (Γ : HOL_ctx n) (φ : tm n),
+    Γ ⊢⟨ n ⟩ φ ~: ℙₛ -> Γ ⊢⟨ n ⟩ ¬ₛ φ ~: ℙₛ.
+Proof.
+  intros. constructor. apply H. apply typ_false.
+Qed.
+
+Definition proof_ctx (n : nat) (Γ : HOL_ctx n) := list (tm n).
+
+Inductive wt_ctx {n : nat} {Γ : HOL_ctx n} : proof_ctx n Γ -> Prop :=
 | wt_nil : wt_ctx nil
-| wt_cons : forall {Ξ : proof_ctx n} {φ : tm n},
+| wt_cons : forall {Ξ : proof_ctx n Γ} {φ : tm n},
     wt_ctx Ξ -> (Γ ⊢⟨ n ⟩ φ ~: ℙₛ) -> wt_ctx (φ :: Ξ).
+
+Inductive proving : forall (n : nat) (Γ : HOL_ctx n)
+                           (Ξ : proof_ctx n Γ) (φ : tm n), Prop :=
+| ax : forall {n : nat} {Γ : HOL_ctx n}
+              {Ξ : proof_ctx n Γ} {φ : tm n},
+    wt_ctx Ξ -> In φ Ξ -> proving n Γ Ξ φ
+| abs : forall {n : nat} {Γ : HOL_ctx n}
+               {Ξ : proof_ctx n Γ} {φ ψ : tm n},
+    proving n Γ (φ :: Ξ) ψ -> proving n Γ Ξ (φ ⇒ₛ ψ)
+| app : forall {n : nat} {Γ : HOL_ctx n}
+               {Ξ : proof_ctx n Γ} {φ ψ : tm n},
+    proving n Γ Ξ (φ ⇒ₛ ψ) -> proving n Γ Ξ φ ->
+    proving n Γ Ξ ψ
+| abs_f : forall {n : nat} {Γ : HOL_ctx n} {Ξ : proof_ctx n Γ}
+                 {φ : tm (S n)} {s : st},
+    proving (S n) (s .: Γ) (List.map (ren_tm shift) Ξ) φ ->
+    proving n Γ Ξ (∀ₛ s φ)
+| app_f : forall {n : nat} {Γ : HOL_ctx n} {Ξ : proof_ctx n Γ}
+                 {φ : tm (S n)} {t : tm n} {s : st},
+    proving n Γ Ξ (∀ₛ s φ) -> Γ ⊢⟨ n ⟩ t ~: s ->
+    proving n Γ Ξ (φ [t .: (fun v => ⟦ v ⟧ₛ)]).
+
+Lemma wt_proving :
+  forall (n : nat) (Γ : HOL_ctx n) (Ξ : proof_ctx n Γ) (φ : tm n),
+    proving n Γ Ξ φ -> wt_ctx Ξ /\ (Γ ⊢⟨ n ⟩ φ ~: ℙₛ).
+Proof.
+  intros. induction H.
+  - split. apply H. induction Ξ. inversion H0.
+    simpl in H0. destruct H0. subst. inversion H. apply H3.
+    inversion H. apply IHΞ. apply H3. apply H0.
+  - destruct IHproving as [wtφΞ wtψ].
+    inversion wtφΞ. subst.
+    split; [exact H2 | constructor ; [apply H3 | apply wtψ]].
+  - destruct IHproving1 as [wtΞ wtψ].
+    dependent destruction wtψ. split. apply wtΞ.
+    apply wtψ2.
+  - destruct IHproving. split.
+    + clear φ H H1. induction Ξ. constructor.
+      inversion H0. constructor. apply (IHΞ H2).
+      admit.
+    + apply (typ_forall s). apply H1.
+  - destruct IHproving. split. apply H1.
+    apply (comp_typ_vec _ _ _ _ (s .: Γ)).
+    asimpl. intro f; case f eqn:e.
+    asimpl. apply typ_var. asimpl. apply H0.
+    dependent destruction H2. apply H2.
+Admitted.
+
+Lemma ren_proof :
+  forall (n m : nat) (Γ : HOL_ctx n) (Δ : HOL_ctx m)
+         (Ξ : proof_ctx n Γ) (φ : tm n) (ξ : fin n -> fin m),
+    (forall f, (ξ >> Δ) f = Γ f) ->
+    proving n Γ Ξ φ -> proving m Δ (map (ren_tm ξ) Ξ) (ren_tm ξ φ).
+Proof.
+  intros. induction H0.
+  - induction Ξ.
+    + inversion H1.
+    + inversion H0; subst. specialize (IHΞ H4).
+      destruct H1.
+      ++ subst. simpl. constructor.
+         constructor. admit.
+         apply (typ_ren m n ξ Δ Γ φ ℙₛ H H5). constructor.
+         reflexivity.
+      ++ specialize (IHΞ H1). simpl. constructor.
+         admit. admit.
+
+Theorem typ_ren :
+  forall (n m : nat) (ξ : fin m -> fin n) (Γ : HOL_ctx n) (Δ : HOL_ctx m)
+         (t : tm m) (s : st),
+    (forall f, (ξ >> Γ) f = Δ f) ->
+    Δ ⊢⟨ m ⟩ t ~: s -> Γ ⊢⟨ n ⟩ ren_tm ξ t ~: s.
+    proving n Γ Ξ φ ->
